src/Pyrosome/Gluing/Dtt/RigidOk.v
@@ -8,7 +8,7 @@ Open Scope list.
 From Utils Require Import Utils.
 From Pyrosome Require Import Theory.Core.
 From Pyrosome.Gluing Require Import CutTModel Eval CutModelSound.
-Require Import Pyrosome.Gluing.Dtt.Syntax Pyrosome.Gluing.Dtt.NormalForms Pyrosome.Gluing.Dtt.Erase Pyrosome.Gluing.Dtt.Rigid.
+Require Import Pyrosome.Gluing.Dtt.Syntax Pyrosome.Gluing.Dtt.NormalForms Pyrosome.Gluing.Dtt.Rigid.
 Import Core.Notations.
 
 (* =====================================================================
